Prove some permutation reduction lemmas

JaEval.v
@@ -184,17 +184,25 @@ Proof.
 Admitted.
 
 (* ======================= Evaluation on extended heap ======================= *)
+Fixpoint ValsPermuted vs vs' pi :=
+  match (vs, vs') with
+  | ([], []) => True
+  | (JFVLoc v::vs, JFVLoc v'::vs') => PiMapsTo v v' pi /\ ValsPermuted vs vs' pi
+  | _ => False
+  end.
+
 Fixpoint ExprsPermuted e e' pi :=
   match (e, e') with
   | (JFNew _ _ vs, JFNew _ _ vs') =>
-      True (* TODO *)
-  | (JFLet _ _ e1 e2, JFLet _ _ e1' e2') =>
+      ValsPermuted vs vs' pi
+  | (JFLet cn x e1 e2, JFLet cn' x' e1' e2') =>
+      cn = cn' /\ x = x' /\
       ExprsPermuted e1 e1' pi /\ ExprsPermuted e2 e2' pi
   | (JFIf (JFVLoc v1) (JFVLoc v2) e1 e2, JFIf (JFVLoc v1') (JFVLoc v2') e1' e2') =>
       ExprsPermuted e1 e1' pi /\ ExprsPermuted e2 e2' pi /\
       PiMapsTo v1 v1' pi /\ PiMapsTo v2 v2' pi
-  | (JFInvoke (JFVLoc v1) _ vs, JFInvoke (JFVLoc v1') _ vs') =>
-      True (* TODO *)
+  | (JFInvoke (JFVLoc v1) m vs, JFInvoke (JFVLoc v1') m' vs') =>
+      PiMapsTo v1 v1' pi /\ ValsPermuted vs vs' pi /\ m = m'
   | (JFAssign ((JFVLoc v1), _) (JFVLoc v2), JFAssign ((JFVLoc v1'), _) (JFVLoc v2')) =>
       PiMapsTo v1 v1' pi /\ PiMapsTo v2 v2' pi
   | (JFVal1 (JFVLoc v1), JFVal1 (JFVLoc v1')) =>
@@ -210,8 +218,8 @@ Fixpoint ExprsPermuted e e' pi :=
 
 Definition CtxPermuted ctx ctx' pi :=
   match (ctx, ctx') with
-  | (JFCtxLet _ _ _ e2, JFCtxLet _ _ _ e2') => ExprsPermuted e2 e2' pi
-  | (JFCtxTry _ _ _ _ e2, JFCtxTry _ _ _ _ e2') => ExprsPermuted e2 e2' pi
+  | (JFCtxLet cn x _ e2, JFCtxLet cn' x' _ e2') => cn = cn' /\ x = x' /\ ExprsPermuted e2 e2' pi
+  | (JFCtxTry _ _ cn x e2, JFCtxTry _ _ cn' x' e2') => cn = cn' /\ x = x' /\ ExprsPermuted e2 e2' pi
   | _ => False
   end.
 
@@ -247,6 +255,32 @@ Proof.
   now apply pi2_pi3, pi1_pi2.
 Qed.
 
+Lemma PiMapsToEqIff : forall l1 l2 l1' l2' pi,
+  Bijection pi ->
+  PiMapsTo l1 l1' pi ->
+  PiMapsTo l2 l2' pi ->
+  (l1 = l2 <-> l1' = l2').
+Proof.
+  intros l1 l2 l1' l2' pi bijection pi_l1 pi_l2.
+  split.
+  + intros l_eq.
+    unfold PiMapsTo in *.
+    destruct l1, l2, l1', l2'; try easy.
+    injection l_eq as n_eq.
+    rewrite <-n_eq in pi_l2.
+    assert (n1_eq := MapsToEq (fst pi) n n1 n2 pi_l1 pi_l2).
+    now rewrite n1_eq.
+  + intros l_eq.
+    unfold PiMapsTo in *.
+    destruct l1, l2, l1', l2'; try easy.
+    apply bijection in pi_l1.
+    apply bijection in pi_l2.
+    injection l_eq as n1_eq.
+    rewrite <-n1_eq in pi_l2.
+    assert (n_eq := MapsToEq (snd pi) n1 n n0 pi_l1 pi_l2).
+    now rewrite n_eq.
+Qed.
+
 Lemma ExistsPermutedResult : forall res A stn_ext pi',
   StacksPermuted [ [] [[JFVal1 (JFVLoc res) ]]_ A] stn_ext pi' ->
   exists res', PiMapsTo res res' pi' /\
@@ -269,7 +303,211 @@ Proof.
   now rewrite A_eq.
 Qed.
 
+Lemma PermutationPreservesClassName : forall h0 h0' h0_perm h0_ext n n_perm C pi,
+  PiMapsTo (JFLoc n) (JFLoc n_perm) pi ->
+  HeapsPermuted h0 h0_perm pi ->
+  JFIDisjointUnion h0_perm h0' h0_ext ->
+  getClassName h0 n = Some C ->
+  getClassName h0_ext n_perm = Some C.
+Proof.
+  intros h0 h0' h0_perm h0_ext n n_perm C pi.
+  intros pi_n pi_h union class_name.
+  unfold getClassName in *.
+  assert (exists o, Heap.find n h0 = Some o).
+    destruct (Heap.find n h0); try discriminate class_name.
+    now exists o.
+  destruct H as (o & n_o_h).
+  rewrite n_o_h in class_name.
+  destruct pi_h as (_ & locs_fst & _ & objs).
+  unfold PiMapsTo in pi_n.
+  assert (n_in_h : Heap.In n h0).
+    apply HeapFacts.elements_in_iff.
+    exists o.
+    now apply HeapFacts.elements_mapsto_iff, HeapFacts.find_mapsto_iff.
+  destruct (locs_fst n n_in_h) as (n_perm' & n_nperm'_pi & n_perm'_in_h_perm).
+  rewrite <-(MapsToEq (fst pi) n n_perm n_perm') in *; trivial.
+  apply HeapFacts.elements_in_iff in n_perm'_in_h_perm.
+  destruct n_perm'_in_h_perm as (o' & n'_o'_h').
+  apply HeapFacts.elements_mapsto_iff in n'_o'_h'.
+
+  apply HeapFacts.find_mapsto_iff in n_o_h.
+  destruct o as (o & cn), o' as (o' & cn').
+  injection class_name as C_eq.
+  destruct (objs n n_perm o cn o' cn') as (cn_eq & _); trivial.
+
+  apply HeapFacts.find_mapsto_iff in n_o_h.
+  assert (subheap : JFISubheap h0_perm h0_ext). apply union.
+  assert (n'_o'_h_ext := subheap n_perm (o', cn') n'_o'_h').
+  apply HeapFacts.find_mapsto_iff in n'_o'_h_ext.
+  now rewrite n'_o'_h_ext, <-cn_eq, C_eq.
+Qed.
+
+Lemma ExistsPermutedExpr : forall e pi,
+  exists e', ExprsPermuted e e' pi.
+Proof.
+Admitted.
+
+Lemma PermutationPreservesSubstExpr : forall e e' pi f l l' e_body e_body',
+  ExprsPermuted e_body e_body' pi ->
+  ExprsPermuted e e' pi ->
+  PiMapsTo l l' pi ->
+  substExpr f l e_body = e ->
+  substExpr f l' e_body' = e'.
+Proof.
+Admitted.
+
+Lemma SubstPermutedExpr : forall f l l' e e' pi,
+  ExprsPermuted e e' pi ->
+  PiMapsTo l l' pi ->
+  ExprsPermuted (substExpr f l e) (substExpr f l' e') pi.
+Proof.
+Admitted.
+
+Lemma PermutationPreservesSubstList : forall fs vs vs',
+  (forall f, In f fs -> f <> JFThis) ->
+  length fs = length vs ->
+  length vs = length vs' -> forall e_body e_body' n n' e pi,
+  ValsPermuted vs vs' pi ->
+  ExprsPermuted e_body e_body' pi ->
+  PiMapsTo (JFLoc n) (JFLoc n') pi ->
+  substList fs vs  (substExpr JFThis (JFLoc n) e_body) = Some e ->
+  exists e',
+  ExprsPermuted e e' pi /\
+  substList fs vs' (substExpr JFThis (JFLoc n') e_body') = Some e'.
+Proof.
+  intros fs vs vs' fs_not_this fs_length_eq vs_length_eq.
+  set (_fs := fs).
+  replace fs with _fs in fs_not_this; try now unfold _fs.
+  set (_vs := vs).
+  set (_vs' := vs').
+  replace _fs  with (fst (split (combine fs (combine vs vs')))) in *.
+  replace _vs  with (fst (split (snd (split (combine fs (combine vs vs')))))).
+  replace _vs' with (snd (split (snd (split (combine fs (combine vs vs')))))).
+  clear fs_length_eq vs_length_eq _fs _vs _vs'.
+  induction (combine fs (combine vs vs')); clear fs vs vs'.
+  + intros e_body e_body' n n' e pi.
+    intros pi_vs pi_body pi_n subst.
+    simpl in *.
+         destruct (ExistsPermutedExpr e pi) as (e' & pi_e).
+    exists e'.
+    split; trivial.
+    unfold substList in *.
+    injection subst as subst.
+    apply PermutationPreservesSubstExpr
+      with (e' := e') (e_body' := e_body') (l' := (JFLoc n')) (pi := pi) in subst; trivial.
+    now rewrite subst.
+  + intros e_body e_body' n n' e pi.
+    intros pi_vs pi_body pi_n subst.
+    destruct a as (f & (v & v')).
+    simpl in *.
+    destruct (split l) as (fs & vs_vs').
+    unfold fst, snd in *.
+    simpl in *.
+    unfold fst, snd in *.
+    destruct (split vs_vs') as (vs & vs').
+    destruct v; try discriminate subst.
+    destruct v'; try destruct pi_vs.
+    assert (next_f_not_this : (forall f : JFRef, In f fs -> f <> JFThis)).
+      intros f0 f0_in_fs. apply (fs_not_this f0). now apply or_intror.
+    rewrite SubstExprComm in subst; [ | now apply fs_not_this, or_introl].
+    destruct (IHl next_f_not_this (substExpr f l0 e_body) (substExpr f l1 e_body') n n' e pi)
+      as (e' & pi_e & subst'); trivial.
+    now apply SubstPermutedExpr.
+    rewrite SubstExprComm in subst'; [ | now apply neq_symmetry, fs_not_this, or_introl].
+    now exists e'.
+  + rewrite combine_split; trivial.
+    ++ unfold snd.
+       rewrite combine_split; trivial.
+    ++ rewrite combine_length.
+       rewrite <-vs_length_eq, <-fs_length_eq.
+       now rewrite min_r.
+  + rewrite combine_split; trivial.
+    ++ unfold snd.
+       rewrite combine_split; trivial.
+    ++ rewrite combine_length.
+       rewrite <-vs_length_eq, <-fs_length_eq.
+       now rewrite min_r.
+  + rewrite combine_split; trivial.
+    rewrite combine_length.
+    rewrite <-vs_length_eq, <-fs_length_eq.
+    now rewrite min_r.
+Qed.
+
+Lemma PermutedValsLengthEq: forall vs vs' pi,
+  ValsPermuted vs vs' pi ->
+  length vs = length vs'.
+Proof.
+Admitted.
+
+Lemma ExistsPermutedBody : forall CC h0 h0' h0_ext h0_perm n n_perm m vs vs_perm ctxs ctxs_perm st st_perm h' st' pi,
+  HeapsPermuted h0 h0_perm pi ->
+  PiMapsTo (JFLoc n) (JFLoc n_perm) pi ->
+  ValsPermuted vs vs_perm pi ->
+  CtxsPermuted ctxs ctxs_perm pi ->
+  StacksPermuted st st_perm pi ->
+  JFIDisjointUnion h0_perm h0' h0_ext ->
+  getInvokeBody CC (getClassName h0 n) n m vs h0 ctxs st = Some (h', st') ->
+  h' = h0 /\
+  exists st'_perm,
+    StacksPermuted st' st'_perm pi  /\
+    getInvokeBody CC (getClassName h0_ext n_perm) n_perm m vs_perm h0_ext ctxs_perm st_perm = Some (h0_ext, st'_perm).
+Proof.
+  intros CC h0 h0' h0_ext h0_perm n n_perm m vs vs_perm ctxs ctxs_perm st st_perm h' st' pi.
+  intros pi_h pi_n pi_vs pi_ctxs pi_st union invoke.
+  unfold getInvokeBody in invoke.
+  assert (exists C, getClassName h0 n = Some C).
+    destruct (getClassName h0 n); try discriminate invoke.
+    now exists j.
+  destruct H as (C & class_name).
+  rewrite class_name in invoke.
+  assert (exists md, methodLookup CC C m = Some md).
+    destruct (methodLookup CC C m); try discriminate invoke.
+    now exists j.
+  destruct H as (md & method_lookup).
+  rewrite method_lookup in invoke.
+  assert (exists Es, substList (map JFVar (params_of_md md)) vs
+             (substExpr JFThis (JFLoc n) (body_of_md md)) = Some Es).
+    destruct (substList (map JFVar (params_of_md md)) vs
+             (substExpr JFThis (JFLoc n) (body_of_md md))); try discriminate invoke.
+    now exists j.
+  destruct H as (Es, subst_method).
+  rewrite subst_method in invoke.
+  injection invoke.
+  intros st_eq h_eq.
+  symmetry in h_eq.
+  split; trivial.
+  destruct st'; try discriminate st_eq.
+  destruct st'; try discriminate st_eq.
+  injection st_eq; clear st_eq.
+  intros st_eq invoke_eq es_eq.
+  rewrite <-st_eq, <-es_eq, <-invoke_eq.
+  assert (fs_not_this : forall f, In f (map JFVar (params_of_md md)) -> f <> JFThis).
+    intros f1 f1_in_map f1_this.
+    apply in_map_iff in f1_in_map.
+    destruct f1_in_map as (x & f1_var & _).
+    now rewrite f1_this in f1_var.
+  assert (fs_length_eq : length (map JFVar (params_of_md md)) = length vs).
+    rewrite map_length.
+    admit. (* TODO params length *)
+  assert (vs_length_eq : length vs = length vs_perm).
+    now apply PermutedValsLengthEq with (pi := pi).
+  assert (pi_body : ExprsPermuted (body_of_md md) (body_of_md md) pi).
+    admit. (* TODO body permuted -- no locs in it *)
+  destruct (PermutationPreservesSubstList (map JFVar (params_of_md md)) vs vs_perm fs_not_this fs_length_eq vs_length_eq (body_of_md md) (body_of_md md) n n_perm Es pi)
+    as (Es_perm & pi_es & subst_perm); trivial.
+  exists (([] [[ Es_perm ]]_ None)
+        :: (ctxs_perm [[JFInvoke (JFVLoc (JFLoc n_perm)) m vs_perm
+            ]]_ None) :: st_perm).
+  split; try easy.
+  apply PermutationPreservesClassName
+    with (h0' := h0') (h0_perm := h0_perm) (h0_ext := h0_ext)
+         (n_perm := n_perm) (pi := pi) in class_name; trivial.
+  unfold getInvokeBody.
+  now rewrite class_name, method_lookup, subst_perm.
+Admitted.
+
 Lemma ReductionPreservesHeapPermutation : forall h0 h0_perm h0' h0_ext st h' st' st_perm pi CC,
+  PiMapsTo (JFLoc NPE_object_loc) (JFLoc NPE_object_loc) pi ->
   StacksPermuted st st_perm pi ->
   HeapsPermuted h0 h0_perm pi ->
   red CC (h0, st) = Some (h', st') ->
@@ -281,6 +519,108 @@ Lemma ReductionPreservesHeapPermutation : forall h0 h0_perm h0' h0_ext st h' st'
     JFIDisjointUnion h'_perm h0' h'_ext /\
     red CC (h0_ext, st_perm) = Some (h'_ext, st'_perm).
 Proof.
+  intros h0 h0_perm h0' h0_ext st h' st' st_perm pi CC.
+  intros pi_npe pi_st pi_h0 red_st union.
+  unfold red in red_st.
+  destruct st; try discriminate red_st.
+  destruct f, E; try discriminate red_st.
+  + admit.
+  + simpl in pi_st.
+    destruct st_perm; [ destruct pi_st |].
+    destruct pi_st as (pi_f & pi_st).
+    unfold FramesPermuted in pi_f.
+    destruct f.
+    destruct pi_f as (pi_let & pi_ctx & A_eq).
+    simpl in pi_let.
+    destruct E; try now destruct pi_let.
+    destruct pi_let as (cn_eq & x_eq & pi_e1 & pi_e2).
+    destruct A.
+      destruct Ctx; try destruct j0; try discriminate red_st.
+    assert (Some (h0, Ctx _[ JFCtxLet cn x __ E2 _[[_ E1 _]]_ None ]_ :: st)
+              = Some (h', st')).
+      now destruct Ctx; try destruct j.
+    injection H.
+    intros st_eq h_eq.
+    exists h0_perm, h0_ext, (Ctx0 _[ JFCtxLet cn x __ E4 _[[_ E3  _]]_ None]_ :: st_perm), pi.
+    rewrite <-st_eq, <-h_eq.
+    split; [ | split; [ | split; [| split]]]; try easy.
+    rewrite <-A_eq, cn_eq, x_eq.
+    now destruct Ctx0; try destruct j.
+  + simpl in pi_st.
+    destruct st_perm; [ destruct pi_st |].
+    destruct pi_st as (pi_f & pi_st).
+    unfold FramesPermuted in pi_f.
+    destruct f.
+    destruct pi_f as (pi_if & pi_ctx & A_eq).
+    simpl in pi_if.
+    destruct v1, v2, E; try destruct v1, v2; try now destruct pi_if.
+    destruct pi_if as (pi_e1 & pi_e2 & pi_l & pi_l0).
+    destruct A.
+      destruct Ctx; try destruct j0; try discriminate red_st.
+    destruct (Classical_Prop.classic (l = l0)) as [l_eq | l_neq].
+   ++ Loc_dec_eq l l0 l_eq.
+      assert (l1_eq : l1 = l2).
+        now apply (PiMapsToEqIff l l0 l1 l2 pi (proj1 pi_h0)).
+      assert (Some (h0, (Ctx [[ E1 ]]_ None) :: st) = Some (h', st')).
+        now destruct Ctx; try destruct j.
+      injection H.
+      intros st_eq h_eq.
+      exists h0_perm, h0_ext, (Ctx0[[ E3 ]]_ None :: st_perm), pi.
+      rewrite <-st_eq, <-h_eq, <-A_eq.
+      split; [ | split; [ | split; [| split]]]; try easy.
+      simpl.
+      Loc_dec_eq l1 l2 l1_eq.
+      now destruct Ctx0; try destruct j.
+   ++ Loc_dec_neq l l0 l_neq.
+      assert (l1_neq : l1 <> l2).
+        intros l1_eq. apply l_neq.
+        now apply (PiMapsToEqIff l l0 l1 l2 pi (proj1 pi_h0)).
+      assert (Some (h0, (Ctx [[ E2 ]]_ None) :: st) = Some (h', st')).
+        now destruct Ctx; try destruct j.
+      injection H.
+      intros st_eq h_eq.
+      exists h0_perm, h0_ext, (Ctx0[[ E4 ]]_ None :: st_perm), pi.
+      rewrite <-st_eq, <-h_eq, <-A_eq.
+      split; [ | split; [ | split; [| split]]]; try easy.
+      simpl.
+      Loc_dec_neq l1 l2 l1_neq.
+      now destruct Ctx0; try destruct j.
+  + simpl in pi_st.
+    destruct st_perm; [ destruct pi_st |].
+    destruct pi_st as (pi_f & pi_st).
+    unfold FramesPermuted in pi_f.
+    destruct f.
+    destruct pi_f as (pi_invoke & pi_ctx & A_eq).
+    simpl in pi_invoke.
+    destruct v, E; try destruct v; try now destruct pi_invoke.
+    destruct pi_invoke as (pi_l & pi_vs & m_eq).
+    destruct A.
+      destruct Ctx, l; try destruct j0; try discriminate red_st.
+    destruct l.
+    ++ assert (Some (h0, (Ctx [[JFVal1 NPE_val ]]_ NPE_mode) :: st) = Some (h', st')).
+         now destruct Ctx; try destruct j.
+       assert (l0_eq : l0 = null).
+         now destruct l0; try destruct pi_l.
+       injection H; intros h_eq st_eq.
+       exists h0_perm, h0_ext, (Ctx0 [[ JFVal1 NPE_val ]]_ NPE_mode :: st_perm), pi.
+       rewrite <-st_eq, <-h_eq, <-A_eq, l0_eq.
+       split; [ | split; [ | split; [| split]]]; try easy.
+       now destruct Ctx0; try destruct j.
+    ++ assert (getInvokeBody CC (getClassName h0 n) n m vs h0 Ctx st = Some (h', st')).
+         now destruct Ctx; try destruct j.
+       destruct l0; try now destruct pi_l.
+       assert (ASdf := ExistsPermutedBody).
+       destruct (ExistsPermutedBody CC h0 h0' h0_ext h0_perm n n0 m vs vs0 Ctx Ctx0 st st_perm h' st' pi)
+         as (h_eq & st'_perm & pi_st' & invoke); trivial.
+       exists h0_perm, h0_ext, st'_perm, pi.
+       rewrite h_eq, <-A_eq, <-m_eq.
+       split; [ | split; [ | split; [| split]]]; try easy.
+       now destruct Ctx0; try destruct j; simpl.
+  + admit.
+  + admit.
+  + admit.
+  + admit.
+  + admit.
 Admitted.
 
 Lemma PermutationEvalAux1 : forall h st confs hn stn CC,
@@ -311,6 +651,7 @@ Proof.
 Qed.
 
 Lemma PartialEvaluationOnExtendedHeap : forall confs h0 h0_perm h0' h0_ext st st_ext hn stn pi CC,
+  PiMapsTo (JFLoc NPE_object_loc) (JFLoc NPE_object_loc) pi ->
   StacksPermuted st st_ext pi ->
   HeapsPermuted h0 h0_perm pi ->
   JFIPartialEval h0 st confs hn stn CC ->
@@ -325,7 +666,7 @@ Proof.
   intros confs.
   induction confs.
   + intros h0 h0_perm h0' h0_ext st st_ext hn stn pi CC.
-    intros pi_h pi_st eval union.
+    intros pi_npe pi_h pi_st eval union.
     unfold JFIPartialEval in eval.
     destruct eval as (h0_eq & st_eq).
     exists [], h0_perm, h0_ext, st_ext, pi.
@@ -333,7 +674,7 @@ Proof.
     ++ now rewrite <-h0_eq.
     ++ now rewrite <-st_eq.
   + intros h0 h0_perm h0' h0_ext st st_ext hn stn pi CC.
-    intros pi_h pi_st eval union.
+    intros pi_npe pi_h pi_st eval union.
     unfold JFIPartialEval in eval.
     fold JFIPartialEval in eval.
     destruct a.
@@ -344,6 +685,7 @@ Proof.
     destruct (IHconfs h' h'_perm h0' h'_ext st' st'_perm hn stn pi' CC)
       as (confs_ext & hn_perm & hn_ext & stn_ext & pin &
           pi'_subset & pin_hn & pin_stn & union_n & eval_rest); trivial.
+      now apply pi_subset.
     exists ((h0_ext,st_ext)::confs_ext), hn_perm, hn_ext, stn_ext, pin.
     split; [ | split; [ | split; [ | split]]]; trivial.
     now apply PermutationSubsetTrans with (pi2 := pi').
@@ -372,6 +714,7 @@ Proof.
   assert (pi_st : StacksPermuted 
     [ [] [[ JFIExprSubstituteEnv env e ]]_ None]
     [ [] [[ JFIExprSubstituteEnv env e ]]_ None] pi). admit.
+  assert (pi_npe : PiMapsTo (JFLoc NPE_object_loc) (JFLoc NPE_object_loc) pi). admit.
 
   destruct (PartialEvaluationOnExtendedHeap confs h0 h0 h0' h0_ext 
     [ [] [[JFIExprSubstituteEnv env e ]]_ None]
